linking_wp: cleanup and add administrative wp rules

theories/interop/linking_wp.v
@@ -92,38 +92,38 @@ Proof using.
 Qed.
 
 Lemma link_at_boundary st :
-  link_state_interp st ∗ link_state_frag Boundary -∗
+  link_state_interp st -∗ link_state_frag Boundary -∗
   ⌜∃ pubσ privσ1 privσ2, st = Link.St pubσ privσ1 privσ2⌝.
 Proof using.
-  iIntros "[Hst Hb]". destruct st; eauto.
+  iIntros "Hst Hb". destruct st; eauto.
   all: iDestruct "Hst" as "(Hb' & _)".
   all: by iDestruct (excl_auth_eq with "Hb Hb'") as %?.
 Qed.
 
 Lemma link_at_in1 st :
-  link_state_interp st ∗ link_state_frag In1 -∗
+  link_state_interp st -∗ link_state_frag In1 -∗
   ⌜∃ σ1 privσ2, st = Link.St1 σ1 privσ2⌝.
 Proof using.
-  iIntros "[Hst Hb]". destruct st; eauto.
+  iIntros "Hst Hb". destruct st; eauto.
   all: iDestruct "Hst" as "(Hb' & ?)".
   all: by iDestruct (excl_auth_eq with "Hb Hb'") as %?.
 Qed.
 
 Lemma link_at_in2 st :
-  link_state_interp st ∗ link_state_frag In2 -∗
+  link_state_interp st -∗ link_state_frag In2 -∗
   ⌜∃ privσ1 σ2, st = Link.St2 privσ1 σ2⌝.
 Proof using.
-  iIntros "[Hst Hb]". destruct st; eauto.
+  iIntros "Hst Hb". destruct st; eauto.
   all: iDestruct "Hst" as "(Hb' & ?)".
   all: by iDestruct (excl_auth_eq with "Hb Hb'") as %?.
 Qed.
 
-Program Instance link_mlangGS : mlangGS hlc val Σ (link_lang Λ1 Λ2) := {
+Global Program Instance link_mlangGS : mlangGS hlc val Σ (link_lang Λ1 Λ2) := {
   state_interp := link_state_interp;
   at_boundary := link_in_state Boundary;
 }.
 
-Program Instance link_linkableGS : linkableGS (link_lang Λ1 Λ2) public_state_interp := {
+Global Program Instance link_linkableGS : linkableGS (link_lang Λ1 Λ2) public_state_interp := {
   private_state_interp := (λ '(privσ1, privσ2),
     own linkG_γ (●E Boundary) ∗
     private_state_interp privσ1 ∗ private_state_interp privσ2)%I;
@@ -138,7 +138,7 @@ Next Obligation.
 Qed.
 Next Obligation.
   iIntros (σ) "(Hb & ? & ?) Hσ".
-  iDestruct (link_at_boundary with "[$Hb $Hσ]") as %(? & ? & ? & ->).
+  iDestruct (link_at_boundary with "Hσ Hb") as %(? & ? & ? & ->).
   iPureIntro. eexists _, _. constructor.
 Qed.
 
@@ -168,48 +168,43 @@ Proof using.
   { rewrite lookup_omap /= lookup_fmap. by destruct (pe1 !! fname). }
 Qed.
 
-Definition link_environ
-  (pe1 : prog_environ Λ1)
-  (pe2 : prog_environ Λ2)
-: prog_environ (link_lang Λ1 Λ2) :=
-{|
-  prog := fmap inl (prog pe1) ∪ fmap inr (prog pe2);
-  T := λ fname vs Φ,
-    (⌜prog pe1 !! fname = None ∧ prog pe2 !! fname = None⌝ ∗
-     (T pe1 fname vs Φ ∨ T pe2 fname vs Φ))%I;
-|}.
+Class is_link_environ
+  (pe1 : prog_environ Λ1) (pe2 : prog_environ Λ2)
+  (pe : prog_environ (link_lang Λ1 Λ2))
+:= IsLinkEnviron {
+  is_link_dom_disj : dom (prog pe1) ## dom (prog pe2);
+  is_link_prog : prog pe = fmap inl (prog pe1) ∪ fmap inr (prog pe2);
 
-Class can_link_prog
-  (pe1 : prog_environ Λ1)
-  (pe2 : prog_environ Λ2)
-:= CanLinkProgs {
-  can_link_disj :
-    dom (prog pe1) ## dom (prog pe2);
-  can_link_spec1 fname (func: mlanguage.func Λ2) vs Φ E :
+  is_link_internal1 fname (func: mlanguage.func Λ2) vs Φ E :
     prog pe2 !! fname = Some func →
     T pe1 fname vs Φ -∗
     ∃ e2, ⌜apply_func func vs = Some e2⌝ ∗ ▷
       (at_boundary Λ2 -∗ WP e2 @ pe2; E {{
         λ v, Φ v ∗ at_boundary Λ2 }});
-  can_link_spec2 fname (func: mlanguage.func Λ1) vs Φ E :
+
+  is_link_internal2 fname (func: mlanguage.func Λ1) vs Φ E :
     prog pe1 !! fname = Some func →
     T pe2 fname vs Φ -∗
     ∃ e1, ⌜apply_func func vs = Some e1⌝ ∗ ▷
       (at_boundary Λ1 -∗ WP e1 @ pe1; E {{
         λ v, Φ v ∗ at_boundary Λ1 }});
+
+  is_link_external1 fname vs Φ :
+    prog pe1 !! fname = None →
+    prog pe2 !! fname = None →
+    T pe1 fname vs Φ -∗ T pe fname vs Φ;
+  is_link_external2 fname vs Φ :
+    prog pe1 !! fname = None →
+    prog pe2 !! fname = None →
+    T pe2 fname vs Φ -∗ T pe fname vs Φ;
 }.
 
-Lemma wp_link_call
-  (pe1 : prog_environ Λ1)
-  (pe2 : prog_environ Λ2)
-  E k fn vs (Φ : val → iProp Σ) fname
-:
-  let pe := link_environ pe1 pe2 in
+Lemma wp_link_call (pe : prog_environ (link_lang Λ1 Λ2)) E k fn vs Φ fname :
   prog pe !! fname = Some fn →
-  WP Link.LkE (Link.RunFunction Λ1 Λ2 fn vs) k @ pe; E {{ Φ }} -∗
-  WP Link.LkE (Link.ExprCall Λ1 Λ2 fname vs) k @ pe; E {{ Φ }}.
+  WP Link.LkE (Link.RunFunction fn vs) k @ pe; E {{ Φ }} -∗
+  WP Link.LkE (Link.ExprCall fname vs) k @ pe; E {{ Φ }}.
 Proof using.
-  iIntros (pe Hfn) "Hwp".
+  iIntros (Hfn) "Hwp".
   iApply wp_unfold. rewrite /wp_pre.
   iIntros (σ) "Hσ". iModIntro. iRight; iRight.
   iSplitR.
@@ -220,13 +215,8 @@ Proof using.
   iModIntro. iNext. iModIntro. iExists _, _. iSplitR; first done. iFrame.
 Qed.
 
-Lemma wp_link_run_function_1
-  (pe1 : prog_environ Λ1)
-  (pe2 : prog_environ Λ2)
-  E k2 k fn arg fname (Φ : val → iProp Σ) (Ξ : val → iProp Σ)
-:
-  let pe := link_environ pe1 pe2 in
-  can_link_prog pe1 pe2 →
+Lemma wp_link_run_function_1 pe1 pe2 pe E k2 k fn arg fname Φ Ξ :
+  is_link_environ pe1 pe2 pe →
   prog pe1 !! fname = Some fn →
   link_state_frag Boundary -∗
   at_boundary Λ1 -∗
@@ -234,15 +224,14 @@ Lemma wp_link_run_function_1
   (∀ e1, ⌜apply_func fn arg = Some e1⌝ -∗
          WP e1 @ pe1; E {{ v, Ξ v ∗ at_boundary Λ1 }} -∗
          link_state_frag In1 -∗
-         WP Link.LkE (Link.Expr1 Λ1 Λ2 e1) (inr k2 :: k) @ pe; E {{ Φ }}) -∗
-  WP Link.LkE (Link.RunFunction Λ1 Λ2 (inl fn) arg) (inr k2 :: k) @ pe; E {{ Φ }}.
+         WP Link.LkE (Link.Expr1 e1) (inr k2 :: k) @ pe; E {{ Φ }}) -∗
+  WP Link.LkE (Link.RunFunction (inl fn) arg) (inr k2 :: k) @ pe; E {{ Φ }}.
 Proof using.
-  iIntros (pe Hcan_link Hfn) "Hb Hb1 HTΞ Hwp".
+  iIntros (Hislink Hfn) "Hb Hb1 HTΞ Hwp".
   iApply wp_unfold. rewrite /wp_pre.
-  iIntros (σ) "Hσ". iDestruct (link_at_boundary with "[$Hb $Hσ]") as %(pubσ&privσ1&privσ2&->).
+  iIntros (σ) "Hσ". iDestruct (link_at_boundary with "Hσ Hb") as %(pubσ&privσ1&privσ2&->).
   iRight; iRight.
-  iPoseProof (can_link_spec2 _ _ _ _ E Hfn with "HTΞ") as (? Happlyfunc) "Hwpcall".
-
+  iPoseProof (is_link_internal2 _ _ _ _ E Hfn with "HTΞ") as (? Happlyfunc) "Hwpcall".
   iDestruct "Hσ" as "(Hob & Hpubσ & Hprivσ1 & Hprivσ2)".
   iMod (state_interp_join with "Hpubσ Hprivσ1") as (σ1) "(Hσ1 & %Hsplit)".
   iModIntro. iSplitR.
@@ -256,13 +245,8 @@ Proof using.
   by iApply ("Hwp" with "[] Hwpcall Hb").
 Qed.
 
-Lemma wp_link_run_function_2
-  (pe1 : prog_environ Λ1)
-  (pe2 : prog_environ Λ2)
-  E k1 k fn arg fname (Φ : val → iProp Σ) (Ξ : val → iProp Σ)
-:
-  let pe := link_environ pe1 pe2 in
-  can_link_prog pe1 pe2 →
+Lemma wp_link_run_function_2 pe1 pe2 pe E k1 k fn arg fname Φ Ξ :
+  is_link_environ pe1 pe2 pe →
   prog pe2 !! fname = Some fn →
   link_state_frag Boundary -∗
   at_boundary Λ2 -∗
@@ -270,15 +254,14 @@ Lemma wp_link_run_function_2
   (∀ e2, ⌜apply_func fn arg = Some e2⌝ -∗
          WP e2 @ pe2; E {{ v, Ξ v ∗ at_boundary Λ2 }} -∗
          link_state_frag In2 -∗
-         WP Link.LkE (Link.Expr2 Λ1 Λ2 e2) (inl k1 :: k) @ pe; E {{ Φ }}) -∗
-  WP Link.LkE (Link.RunFunction Λ1 Λ2 (inr fn) arg) (inl k1 :: k) @ pe; E {{ Φ }}.
+         WP Link.LkE (Link.Expr2 e2) (inl k1 :: k) @ pe; E {{ Φ }}) -∗
+  WP Link.LkE (Link.RunFunction (inr fn) arg) (inl k1 :: k) @ pe; E {{ Φ }}.
 Proof using.
-  iIntros (pe Hcan_link Hfn) "Hb Hb2 HTΞ Hwp".
+  iIntros (Hislink Hfn) "Hb Hb2 HTΞ Hwp".
   iApply wp_unfold. rewrite /wp_pre.
-  iIntros (σ) "Hσ". iDestruct (link_at_boundary with "[$Hb $Hσ]") as %(pubσ&privσ1&privσ2&->).
+  iIntros (σ) "Hσ". iDestruct (link_at_boundary with "Hσ Hb") as %(pubσ&privσ1&privσ2&->).
   iRight; iRight.
-  iPoseProof (can_link_spec1 _ _ _ _ E Hfn with "HTΞ") as (? Happlyfunc) "Hwpcall".
-
+  iPoseProof (is_link_internal1 _ _ _ _ E Hfn with "HTΞ") as (? Happlyfunc) "Hwpcall".
   iDestruct "Hσ" as "(Hob & Hpubσ & Hprivσ1 & Hprivσ2)".
   iMod (state_interp_join with "Hpubσ Hprivσ2") as (σ2) "(Hσ2 & %Hsplit)".
   iModIntro. iSplitR.
@@ -292,18 +275,13 @@ Proof using.
   by iApply ("Hwp" with "[] Hwpcall Hb").
 Qed.
 
-Lemma wp_link_retval_1
-  (pe1 : prog_environ Λ1)
-  (pe2 : prog_environ Λ2)
-  E k1 v (Φ : val → iProp Σ)
-:
-  let pe := link_environ pe1 pe2 in
-  (link_state_frag In1 -∗ WP LkSE (Link.Expr1 Λ1 Λ2 (fill k1 (of_val Λ1 v))) @ pe; E {{ Φ }}) -∗
-  (link_state_frag Boundary -∗ WP Link.LkE (Link.ExprV Λ1 Λ2 v) [inl k1] @ pe; E {{ Φ }}).
+Lemma wp_link_retval_1 (pe : prog_environ (link_lang Λ1 Λ2)) E k1 v Φ :
+  (link_state_frag In1 -∗ WP LkSE (Link.Expr1 (fill k1 (of_val Λ1 v))) @ pe; E {{ Φ }}) -∗
+  (link_state_frag Boundary -∗ WP Link.LkE (Link.ExprV v) [inl k1] @ pe; E {{ Φ }}).
 Proof using.
-  iIntros (pe) "Hwp Hb".
+  iIntros "Hwp Hb".
   iApply wp_unfold. rewrite /wp_pre.
-  iIntros (σ) "Hσ". iDestruct (link_at_boundary with "[$Hσ $Hb]") as %(pubσ&privσ1&privσ2&->).
+  iIntros (σ) "Hσ". iDestruct (link_at_boundary with "Hσ Hb") as %(pubσ&privσ1&privσ2&->).
   iDestruct "Hσ" as "(Hob & Hpub & Hpriv1 & Hpriv2)".
   iMod (state_interp_join with "Hpub Hpriv1") as (σ1) "[Hσ1 %Hsplit]".
   iModIntro. iRight. iRight.
@@ -316,18 +294,13 @@ Proof using.
   iModIntro. iExists _, _. iSplitR; first done. iFrame. iApply "Hwp". iFrame.
 Qed.
 
-Lemma wp_link_retval_2
-  (pe1 : prog_environ Λ1)
-  (pe2 : prog_environ Λ2)
-  E k2 v (Φ : val → iProp Σ)
-:
-  let pe := link_environ pe1 pe2 in
-  (link_state_frag In2 -∗ WP LkSE (Link.Expr2 Λ1 Λ2 (fill k2 (of_val Λ2 v))) @ pe; E {{ Φ }}) -∗
-  (link_state_frag Boundary -∗ WP Link.LkE (Link.ExprV Λ1 Λ2 v) [inr k2] @ pe; E {{ Φ }}).
+Lemma wp_link_retval_2 (pe : prog_environ (link_lang Λ1 Λ2)) E k2 v Φ :
+  (link_state_frag In2 -∗ WP LkSE (Link.Expr2 (fill k2 (of_val Λ2 v))) @ pe; E {{ Φ }}) -∗
+  (link_state_frag Boundary -∗ WP Link.LkE (Link.ExprV v) [inr k2] @ pe; E {{ Φ }}).
 Proof using.
-  iIntros (pe) "Hwp Hb".
+  iIntros "Hwp Hb".
   iApply wp_unfold. rewrite /wp_pre.
-  iIntros (σ) "Hσ". iDestruct (link_at_boundary with "[$Hσ $Hb]") as %(pubσ&privσ1&privσ2&->).
+  iIntros (σ) "Hσ". iDestruct (link_at_boundary with "Hσ Hb") as %(pubσ&privσ1&privσ2&->).
   iDestruct "Hσ" as "(Hob & Hpub & Hpriv1 & Hpriv2)".
   iMod (state_interp_join with "Hpub Hpriv2") as (σ2) "[Hσ2 %Hsplit]".
   iModIntro. iRight. iRight.
@@ -340,12 +313,8 @@ Proof using.
   iModIntro. iExists _, _. iSplitR; first done. iFrame. iApply "Hwp". iFrame.
 Qed.
 
-Lemma wp_link_extcall_1
-  (pe1 : prog_environ Λ1)
-  (pe2 : prog_environ Λ2)
-  E k1 fn_name arg (Φ : val → iProp Σ) (Ξ : val → iProp Σ)
-:
-  let pe := link_environ pe1 pe2 in
+Lemma wp_link_extcall_1 pe1 pe2 pe E k1 fn_name arg Φ Ξ :
+  is_link_environ pe1 pe2 pe →
   prog pe1 !! fn_name = None →
   prog pe2 !! fn_name = None →
   T pe1 fn_name arg Ξ -∗
@@ -354,30 +323,26 @@ Lemma wp_link_extcall_1
   (▷ ∀ r, WP fill k1 (of_class Λ1 (ExprVal r)) @ pe1; E {{ λ v, Φ v ∗ at_boundary Λ1 }} -∗
         link_state_frag Boundary -∗
         at_boundary Λ2 -∗
-        WP Link.LkE (Link.ExprV Λ1 Λ2 r) [inl k1] @ pe; E {{ λ v, Φ v ∗ at_boundary (link_lang Λ1 Λ2) }}) -∗
+        WP Link.LkE (Link.ExprV r) [inl k1] @ pe; E {{ λ v, Φ v ∗ at_boundary (link_lang Λ1 Λ2) }}) -∗
   at_boundary (link_lang Λ1 Λ2) -∗
-  WP Link.LkE (Link.ExprCall Λ1 Λ2 fn_name arg) [inl k1] @ pe; E {{ λ v, Φ v ∗ at_boundary (link_lang Λ1 Λ2) }}.
+  WP Link.LkE (Link.ExprCall fn_name arg) [inl k1] @ pe; E {{ λ v, Φ v ∗ at_boundary (link_lang Λ1 Λ2) }}.
 Proof using.
-  iIntros (pe Hfn1 Hfn2) "HTΞ HΞ Hwp (Hb & Hb1 & Hb2)".
+  iIntros (Hislink Hfn1 Hfn2) "HTΞ HΞ Hwp (Hb & Hb1 & Hb2)".
   assert (Hpef: prog pe !! fn_name = None).
-  { apply lookup_union_None. rewrite !lookup_fmap Hfn1 Hfn2 //. }
+  { rewrite is_link_prog. apply lookup_union_None. rewrite !lookup_fmap Hfn1 Hfn2 //. }
   iApply wp_unfold. rewrite /wp_pre.
-  iIntros (σ) "Hσ". iDestruct (link_at_boundary with "[$Hσ $Hb]") as %(pubσ&privσ1&privσ2&->).
+  iIntros (σ) "Hσ". iDestruct (link_at_boundary with "Hσ Hb") as %(pubσ&privσ1&privσ2&->).
   iModIntro. iRight; iLeft. iExists _, _, [inl k1]. iSplitR; [by eauto|].
   iSplitR; first by eauto. iFrame "Hσ Hb Hb1 Hb2". iExists Ξ. iSplitL "HTΞ".
-  { rewrite /pe /=. iSplitR; [now iPureIntro; split; eauto|]. iLeft. iApply "HTΞ". }
+  { by iApply is_link_external1. }
   iNext. iIntros (r) "[Hr Hb]". iDestruct "Hb" as "(Hb & Hb1 & Hb2)".
   simpl.
   iSpecialize ("HΞ" with "[$Hr $Hb1]"). rewrite -fill_comp fill_empty.
   iApply ("Hwp" with "HΞ Hb Hb2").
 Qed.
 
-Lemma wp_link_extcall_2
-  (pe1 : prog_environ Λ1)
-  (pe2 : prog_environ Λ2)
-  E k2 fn_name arg (Φ : val → iProp Σ) (Ξ : val → iProp Σ)
-:
-  let pe := link_environ pe1 pe2 in
+Lemma wp_link_extcall_2 pe1 pe2 pe E k2 fn_name arg Φ Ξ :
+  is_link_environ pe1 pe2 pe →
   prog pe1 !! fn_name = None →
   prog pe2 !! fn_name = None →
   T pe2 fn_name arg Ξ -∗
@@ -386,44 +351,44 @@ Lemma wp_link_extcall_2
   (▷ ∀ r, WP fill k2 (of_class Λ2 (ExprVal r)) @ pe2; E {{ λ v, Φ v ∗ at_boundary Λ2 }} -∗
         link_state_frag Boundary -∗
         at_boundary Λ1 -∗
-        WP Link.LkE (Link.ExprV Λ1 Λ2 r) [inr k2] @ pe; E {{ λ v, Φ v ∗ at_boundary (link_lang Λ1 Λ2) }}) -∗
+        WP Link.LkE (Link.ExprV r) [inr k2] @ pe; E {{ λ v, Φ v ∗ at_boundary (link_lang Λ1 Λ2) }}) -∗
   at_boundary (link_lang Λ1 Λ2) -∗
-  WP Link.LkE (Link.ExprCall Λ1 Λ2 fn_name arg) [inr k2] @ pe; E {{ λ v, Φ v ∗ at_boundary (link_lang Λ1 Λ2) }}.
+  WP Link.LkE (Link.ExprCall fn_name arg) [inr k2] @ pe; E {{ λ v, Φ v ∗ at_boundary (link_lang Λ1 Λ2) }}.
 Proof using.
-  iIntros (pe Hfn1 Hfn2) "HTΞ HΞ Hwp (Hb & Hb1 & Hb2)".
+  iIntros (Hislink Hfn1 Hfn2) "HTΞ HΞ Hwp (Hb & Hb1 & Hb2)".
   assert (Hpef: prog pe !! fn_name = None).
-  { apply lookup_union_None. rewrite !lookup_fmap Hfn1 Hfn2 //. }
+  { rewrite is_link_prog. apply lookup_union_None. rewrite !lookup_fmap Hfn1 Hfn2 //. }
   iApply wp_unfold. rewrite /wp_pre.
-  iIntros (σ) "Hσ". iDestruct (link_at_boundary with "[$Hσ $Hb]") as %(pubσ&privσ1&privσ2&->).
+  iIntros (σ) "Hσ". iDestruct (link_at_boundary with "Hσ Hb") as %(pubσ&privσ1&privσ2&->).
   iModIntro. iRight; iLeft. iExists _, _, [inr k2]. iSplitR; [by eauto|].
   iSplitR; first by eauto. iFrame "Hσ Hb Hb1 Hb2". iExists Ξ. iSplitL "HTΞ".
-  { rewrite /pe /=. iSplitR; [now iPureIntro; split; eauto|]. iRight. iApply "HTΞ". }
+  { by iApply is_link_external2. }
   iNext. iIntros (r) "[Hr Hb]". iDestruct "Hb" as "(Hb & Hb1 & Hb2)".
   simpl.
   iSpecialize ("HΞ" with "[$Hr $Hb2]"). rewrite -fill_comp fill_empty.
   iApply ("Hwp" with "HΞ Hb Hb1").
 Qed.
 
-Lemma link_head_step_call_ext_1_inv pe1 pe2 K f vs σ1 privσ2 X :
-  let pe := link_environ pe1 pe2 in
-  can_link_prog pe1 pe2 →
+Lemma link_head_step_call_ext_1_inv pe1 pe2 pe K f vs σ1 privσ2 X :
+  is_link_environ pe1 pe2 pe →
   prog pe1 !! f = None →
-  head_step (prog pe) (LkSE (Link.Expr1 Λ1 Λ2 (fill K (of_class Λ1 (ExprCall f vs)))),
+  head_step (prog pe) (LkSE (Link.Expr1 (fill K (of_class Λ1 (ExprCall f vs)))),
                        Link.St1 σ1 privσ2) X →
   ∃ pubσ privσ1 k,
     K = comp_ectx k empty_ectx ∧
-    X (Link.LkE (Link.ExprCall Λ1 Λ2 f vs) [inl k], Link.St pubσ privσ1 privσ2) ∧
+    X (Link.LkE (Link.ExprCall f vs) [inl k], Link.St pubσ privσ1 privσ2) ∧
     split_state σ1 pubσ privσ1.
 Proof using.
-  intros pe Hcan_link Hf Hstep. inversion Hstep; subst; simplify_eq.
+  intros Hislink Hf Hstep. inversion Hstep; subst; simplify_eq.
   { exfalso.
     match goal with H:_|-_ => eapply call_prim_step_fill in H as (?&?&HH&?&_) end.
-    rewrite proj1_prog_union in HH; [| apply Hcan_link]. congruence. }
+    rewrite is_link_prog in HH.
+    rewrite proj1_prog_union in HH; [| apply Hislink]. congruence. }
   { exfalso. match goal with H:_|-_ => apply mk_is_Some in H; apply fill_val in H; destruct H as [? HH] end.
     rewrite /to_val to_of_class // in HH. }
   match goal with H: fill _ _ = fill _ _ |- _ => rename H into Hfill end.
   match goal with H: Link.proj1_prog _ _ _ !! _ = None |- _ => rename H into Hnofn end.
-  rewrite proj1_prog_union in Hnofn;[|apply Hcan_link].
+  rewrite is_link_prog proj1_prog_union in Hnofn;[|apply Hislink].
   pose proof (call_in_ctx_to_val _ _ _ _ _ Hfill) as [[K'' ->]|Hval].
   2: { exfalso. unfold to_val in Hval. destruct Hval. by repeat case_match. }
   rewrite -fill_comp in Hfill. apply fill_inj in Hfill. subst e1.
@@ -435,25 +400,24 @@ Proof using.
   rewrite fill_empty to_of_class in Hcall. by simplify_eq/=.
 Qed.
 
-Lemma link_head_step_call_ext_2_inv pe1 pe2 K f vs σ2 privσ1 X :
-  let pe := link_environ pe1 pe2 in
-  can_link_prog pe1 pe2 →
+Lemma link_head_step_call_ext_2_inv pe1 pe2 pe K f vs σ2 privσ1 X :
+  is_link_environ pe1 pe2 pe →
   prog pe2 !! f = None →
-  head_step (prog pe) (LkSE (Link.Expr2 Λ1 Λ2 (fill K (of_class Λ2 (ExprCall f vs)))),
+  head_step (prog pe) (LkSE (Link.Expr2 (fill K (of_class Λ2 (ExprCall f vs)))),
                        Link.St2 privσ1 σ2) X →
   ∃ pubσ privσ2 k,
     K = comp_ectx k empty_ectx ∧
-    X (Link.LkE (Link.ExprCall Λ1 Λ2 f vs) [inr k], Link.St pubσ privσ1 privσ2) ∧
+    X (Link.LkE (Link.ExprCall f vs) [inr k], Link.St pubσ privσ1 privσ2) ∧
     split_state σ2 pubσ privσ2.
 Proof using.
-  intros pe Hcan_link Hf Hstep. inversion Hstep; subst; simplify_eq.
+  intros Hislink Hf Hstep. inversion Hstep; subst; simplify_eq.
   { exfalso. match goal with H:_|-_ => eapply call_prim_step_fill in H as (?&?&HH&?&_) end.
-    rewrite proj2_prog_union in HH; [| apply Hcan_link]. congruence. }
+    rewrite is_link_prog proj2_prog_union in HH; [| apply Hislink]. congruence. }
   { exfalso. match goal with H:_|-_ => apply mk_is_Some in H; apply fill_val in H; destruct H as [? HH] end.
     rewrite /to_val to_of_class // in HH. }
   match goal with H: fill _ _ = fill _ _ |- _ => rename H into Hfill end.
   match goal with H: Link.proj2_prog _ _ _ !! _ = None |- _ => rename H into Hnofn end.
-  rewrite proj2_prog_union in Hnofn;[|apply Hcan_link].
+  rewrite is_link_prog proj2_prog_union in Hnofn;[|apply Hislink].
   pose proof (call_in_ctx_to_val _ _ _ _ _ Hfill) as [[K'' ->]|Hval].
   2: { exfalso. unfold to_val in Hval. destruct Hval. by repeat case_match. }
   rewrite -fill_comp in Hfill. apply fill_inj in Hfill. subst e2.
@@ -465,26 +429,21 @@ Proof using.
   rewrite fill_empty to_of_class in Hcall. by simplify_eq/=.
 Qed.
 
-Lemma wp_link_run
-  (pe1 : prog_environ Λ1)
-  (pe2 : prog_environ Λ2)
-  E
-:
-  let pe := link_environ pe1 pe2 in
-  can_link_prog pe1 pe2 →
+Lemma wp_link_run_mut pe1 pe2 pe E :
+  is_link_environ pe1 pe2 pe →
   ⊢ □ (
     (∀ e1 Φ, WP e1 @ pe1; E {{ λ v, Φ v ∗ at_boundary Λ1 }} -∗ link_in_state In1 -∗
-             WP (LkSE (Link.Expr1 Λ1 Λ2 e1)) @ pe; E {{ λ v, Φ v ∗ link_in_state Boundary }}) ∗
+             WP (LkSE (Link.Expr1 e1)) @ pe; E {{ λ v, Φ v ∗ link_in_state Boundary }}) ∗
     (∀ e2 Φ, WP e2 @ pe2; E {{ λ v, Φ v ∗ at_boundary Λ2 }} -∗ link_in_state In2 -∗
-             WP (LkSE (Link.Expr2 Λ1 Λ2 e2)) @ pe; E {{ λ v, Φ v ∗ link_in_state Boundary }})
+             WP (LkSE (Link.Expr2 e2)) @ pe; E {{ λ v, Φ v ∗ link_in_state Boundary }})
   ).
 Proof using.
-  intros pe Hcan_link. iLöb as "IH". iModIntro. iSplitL.
+  intros Hislink. iLöb as "IH". iModIntro. iSplitL.
   (* Case 1: running Λ1 *)
   { iIntros (e1 Φ) "Hwp [Hb Hb2]".
     rewrite wp_unfold. rewrite /wp_pre.
     iApply wp_unfold. rewrite /wp_pre.
-    iIntros (σ) "Hσ". iDestruct (link_at_in1 with "[$Hb $Hσ]") as %(σ1 & privσ2 & ->).
+    iIntros (σ) "Hσ". iDestruct (link_at_in1 with "Hσ Hb") as %(σ1 & privσ2 & ->).
     iDestruct "Hσ" as "(Hob & Hσ1 & Hpriv2)".
     iMod ("Hwp" $! σ1 with "[$Hσ1]") as "[Hwp|[Hwp|Hwp]]".
 
@@ -493,7 +452,7 @@ Proof using.
       iModIntro. iRight; iRight.
       (* administrative step Val1S: Link.Expr1 ~> Link.ExprV *)
       iDestruct (@splittable_at_boundary with "Hb1 Hσ") as %(pubσ&privσ1&Hsplitσ1).
-      assert (Hhred: head_reducible (prog pe) (LkSE (Link.Expr1 Λ1 Λ2 (of_class Λ1 (ExprVal v)))) (Link.St1 σ1 privσ2)).
+      assert (Hhred: head_reducible (prog pe) (LkSE (Link.Expr1 (of_class Λ1 (ExprVal v)))) (Link.St1 σ1 privσ2)).
       { exists (λ _, True). eapply Link.Val1S; eauto. rewrite /to_val to_of_class //=. }
       iSplitR; [iPureIntro; by apply head_prim_reducible|].
       iIntros (X Hstep). apply head_reducible_prim_step in Hstep; [|done].
@@ -514,9 +473,9 @@ Proof using.
     { iDestruct "Hwp" as (f vs K -> Hf) "(Hb1 & Hσ1 & Hcall)". iModIntro. iRight; iRight.
       (* administrative step MakeCall1S: Link.Expr1 ~> Link.ExprCall *)
       iDestruct (@splittable_at_boundary with "Hb1 Hσ1") as %(pubσ&privσ1&Hsplitσ1).
-      assert (head_reducible (prog pe) (LkSE (Link.Expr1 Λ1 Λ2 (fill K (of_class Λ1 (ExprCall f vs))))) (Link.St1 σ1 privσ2)).
+      assert (head_reducible (prog pe) (LkSE (Link.Expr1 (fill K (of_class Λ1 (ExprCall f vs))))) (Link.St1 σ1 privσ2)).
       { exists (λ _, True). eapply Link.MakeCall1S; eauto. by rewrite to_of_class.
-        rewrite proj1_prog_union; [done | apply Hcan_link]. }
+        rewrite is_link_prog proj1_prog_union; [done | apply Hislink]. }
       iSplitR; [iPureIntro; by apply head_prim_reducible|].
       iIntros (X Hstep). apply head_reducible_prim_step in Hstep;[|done].
       clear pubσ privσ1 Hsplitσ1.
@@ -534,7 +493,7 @@ Proof using.
 
       { (* call to a function of pe2 *)
         assert (prog pe !! f = Some (inr fn2)) as Hpef.
-        { rewrite lookup_union_r lookup_fmap. by rewrite Hf2. by rewrite Hf. }
+        { rewrite is_link_prog lookup_union_r lookup_fmap. by rewrite Hf2. by rewrite Hf. }
 
         (* administrative step CallS: Link.ExprCall ~> LinkRunFunction *)
         iApply wp_link_call; first done.
@@ -542,8 +501,8 @@ Proof using.
         iApply (wp_link_run_function_2 with "Hb Hb2 HTΞ"); first done.
         iIntros (e2 He2) "Hwpcall Hb".
 
-        progress change (Link.LkE (Link.Expr2 Λ1 Λ2 e2) [inl k1]) with
-          (Link.fill _ _ ([inl k1]:ectx (link_lang Λ1 Λ2)) (LkSE (Link.Expr2 Λ1 Λ2 e2))).
+        progress change (Link.LkE (Link.Expr2 e2) [inl k1]) with
+          (Link.fill _ _ ([inl k1]:ectx (link_lang Λ1 Λ2)) (LkSE (Link.Expr2 e2))).
         iApply wp_bind.
         iApply (wp_wand with "[Hwpcall Hb Hb1]").
         { iDestruct "IH" as "#[_ IH2]". iApply ("IH2" with "Hwpcall [$Hb $Hb1]"). }
@@ -567,27 +526,28 @@ Proof using.
 
     { (* WP: step case *)
       iDestruct "Hwp" as (Hred) "Hwp". iModIntro. iRight; iRight.
-      assert (head_reducible (prog pe) (LkSE (Link.Expr1 Λ1 Λ2 e1)) (Link.St1 σ1 privσ2)).
+      assert (head_reducible (prog pe) (LkSE (Link.Expr1 e1)) (Link.St1 σ1 privσ2)).
       { destruct Hred as (? & Hstep). exists (λ _, True).
-        eapply Link.Step1S. rewrite proj1_prog_union; [| apply Hcan_link]. all: eauto. }
+        eapply Link.Step1S. rewrite is_link_prog proj1_prog_union; [| apply Hislink].
+        all: eauto. }
       iSplitR; [by iPureIntro; apply head_prim_reducible|].
       iIntros (X Hstep). apply head_reducible_prim_step in Hstep;[|done].
       inversion Hstep; simplify_eq.
       { (* non-vacuous case: step in Λ1 *)
         clear Hstep. rename H4 into Hstep.
-        rewrite proj1_prog_union in Hstep; [|apply Hcan_link].
+        rewrite is_link_prog proj1_prog_union in Hstep; [|apply Hislink].
         iSpecialize ("Hwp" $! _ Hstep). iMod "Hwp". iIntros "!>!>". iMod "Hwp" as (e' σ' HX) "[Hσ Hwp]".
         iModIntro. iExists _, _. iSplitR; [iPureIntro; naive_solver|]. iFrame "Hσ Hob Hpriv2".
         iDestruct "IH" as "[IH1 _]". iApply ("IH1" with "Hwp [$Hb $Hb2]"). }
       { exfalso. apply reducible_not_val in Hred. congruence. }
       { exfalso. clear Hstep. erewrite <-(of_to_class e0) in Hred; [|eassumption].
-        rewrite proj1_prog_union in H4;[|apply Hcan_link].
+        rewrite is_link_prog proj1_prog_union in H4;[|apply Hislink].
         destruct Hred as (?&Hred). eapply extcall_ctx_irreducible; eauto. } } }
 
   (* Case 2: running Λ2 *)
   { iIntros (e2 Φ) "Hwp [Hb Hb1]".
     rewrite wp_unfold. rewrite /wp_pre. iApply wp_unfold. rewrite /wp_pre.
-    iIntros (σ) "Hσ". iDestruct (link_at_in2 with "[$Hb $Hσ]") as %(privσ1 & σ2 & ->).
+    iIntros (σ) "Hσ". iDestruct (link_at_in2 with "Hσ Hb") as %(privσ1 & σ2 & ->).
     iDestruct "Hσ" as "(Hob & Hpriv1 & Hσ2)".
     iMod ("Hwp" $! σ2 with "[$Hσ2]") as "[Hwp|[Hwp|Hwp]]".
 
@@ -595,7 +555,7 @@ Proof using.
     { iDestruct "Hwp" as (v ->) "[Hσ [HΦ Hb2]]". iModIntro. iRight; iRight.
       (* administrative step Val2S: Link.Expr2 ~> Link.ExprV *)
       iDestruct (@splittable_at_boundary with "Hb2 Hσ") as %(pubσ&privσ2&Hsplitσ2).
-      assert (Hhred: head_reducible (prog pe) (LkSE (Link.Expr2 Λ1 Λ2 (of_class Λ2 (ExprVal v)))) (Link.St2 privσ1 σ2)).
+      assert (Hhred: head_reducible (prog pe) (LkSE (Link.Expr2 (of_class Λ2 (ExprVal v)))) (Link.St2 privσ1 σ2)).
       { exists (λ _, True). eapply Link.Val2S; eauto. rewrite /to_val to_of_class //=. }
       iSplitR; [iPureIntro; by apply head_prim_reducible|].
       iIntros (X Hstep). apply head_reducible_prim_step in Hstep; [|done].
@@ -616,9 +576,9 @@ Proof using.
     { iDestruct "Hwp" as (f vs K -> Hf) "(Hb2 & Hσ2 & Hcall)". iModIntro. iRight; iRight.
       (* administrative step MakeCall1S: Link.Expr2 ~> Link.ExprCall *)
       iDestruct (@splittable_at_boundary with "Hb2 Hσ2") as %(pubσ&privσ2&Hsplitσ2).
-      assert (head_reducible (prog pe) (LkSE (Link.Expr2 Λ1 Λ2 (fill K (of_class Λ2 (ExprCall f vs))))) (Link.St2 privσ1 σ2)).
+      assert (head_reducible (prog pe) (LkSE (Link.Expr2 (fill K (of_class Λ2 (ExprCall f vs))))) (Link.St2 privσ1 σ2)).
       { exists (λ _, True). eapply Link.MakeCall2S; eauto. by rewrite to_of_class.
-        rewrite proj2_prog_union; [done | apply Hcan_link]. }
+        rewrite is_link_prog proj2_prog_union; [done | apply Hislink]. }
       iSplitR; [iPureIntro; by apply head_prim_reducible|].
       iIntros (X Hstep). apply head_reducible_prim_step in Hstep;[|done].
       clear pubσ privσ2 Hsplitσ2.
@@ -636,7 +596,7 @@ Proof using.
 
       { (* call to a function of pe1 *)
         assert (prog pe !! f = Some (inl fn1)) as Hpef.
-        { rewrite lookup_union_l lookup_fmap. by rewrite Hf1. by rewrite Hf. }
+        { rewrite is_link_prog lookup_union_l lookup_fmap. by rewrite Hf1. by rewrite Hf. }
 
         (* administrative step CallS: Link.ExprCall ~> LinkRunFunction *)
         iApply wp_link_call; first done.
@@ -644,8 +604,8 @@ Proof using.
         iApply (wp_link_run_function_1 with "Hb Hb1 HTΞ"); first done.
         iIntros (e1 He1) "Hwpcall Hb".
 
-        progress change (Link.LkE (Link.Expr1 Λ1 Λ2 e1) [inr k2]) with
-          (Link.fill _ _ ([inr k2]:ectx (link_lang Λ1 Λ2)) (LkSE (Link.Expr1 Λ1 Λ2 e1))).
+        progress change (Link.LkE (Link.Expr1 e1) [inr k2]) with
+          (Link.fill _ _ ([inr k2]:ectx (link_lang Λ1 Λ2)) (LkSE (Link.Expr1 e1))).
         iApply wp_bind.
         iApply (wp_wand with "[Hwpcall Hb Hb2]").
         { iDestruct "IH" as "#[IH1 _]". iApply ("IH1" with "Hwpcall [$Hb $Hb2]"). }
@@ -668,23 +628,99 @@ Proof using.
 
     { (* WP: step case *)
       iDestruct "Hwp" as (Hred) "Hwp". iModIntro. iRight; iRight.
-      assert (head_reducible (prog pe) (LkSE (Link.Expr2 Λ1 Λ2 e2)) (Link.St2 privσ1 σ2)).
+      assert (head_reducible (prog pe) (LkSE (Link.Expr2 e2)) (Link.St2 privσ1 σ2)).
       { destruct Hred as (? & Hstep).
-        exists (λ _, True). eapply Link.Step2S. rewrite proj2_prog_union; [| apply Hcan_link].
-        all: eauto. }
+        exists (λ _, True). eapply Link.Step2S.
+        rewrite is_link_prog proj2_prog_union; [| apply Hislink]. all: eauto. }
       iSplitR; [by iPureIntro; apply head_prim_reducible|].
       iIntros (X Hstep). apply head_reducible_prim_step in Hstep;[|done].
       inversion Hstep; simplify_eq.
       { (* non-vacuous case: step in Λ2 *)
         clear Hstep. rename H4 into Hstep.
-        rewrite proj2_prog_union in Hstep; [|apply Hcan_link].
+        rewrite is_link_prog proj2_prog_union in Hstep; [|apply Hislink].
         iSpecialize ("Hwp" $! _ Hstep). iMod "Hwp". iIntros "!>!>". iMod "Hwp" as (e' σ' HX) "[Hσ Hwp]".
         iModIntro. iExists _, _. iSplitR; [iPureIntro; naive_solver|]. iFrame "Hob Hσ Hpriv1".
         iDestruct "IH" as "[_ IH2]". iApply ("IH2" with "Hwp [$Hb $Hb1]"). }
       { exfalso. apply reducible_not_val in Hred. congruence. }
       { exfalso. clear Hstep. erewrite <-(of_to_class e0) in Hred; [|eassumption].
-        rewrite proj2_prog_union in H4;[|apply Hcan_link].
+        rewrite is_link_prog proj2_prog_union in H4;[|apply Hislink].
         destruct Hred as (?&Hred). eapply extcall_ctx_irreducible; eauto. } } }
+Qed.
+
+Lemma wp_link_run1 pe1 pe2 pe E e1 Φ :
+  is_link_environ pe1 pe2 pe →
+  link_in_state In1 -∗
+  WP e1 @ pe1; E {{ λ v, Φ v ∗ at_boundary Λ1 }} -∗
+  WP LkSE (Link.Expr1 e1) @ pe; E {{ λ v, Φ v ∗ link_in_state Boundary }}.
+Proof using.
+  iIntros (Hislink) "Hlkst Hwp". iDestruct (wp_link_run_mut _ _ _ _ Hislink) as "[H _]".
+  iApply ("H" with "Hwp Hlkst").
+Qed.
+
+Lemma wp_link_run2 pe1 pe2 pe E e2 Φ :
+  is_link_environ pe1 pe2 pe →
+  link_in_state In2 -∗
+  WP e2 @ pe2; E {{ λ v, Φ v ∗ at_boundary Λ2 }} -∗
+  WP LkSE (Link.Expr2 e2) @ pe; E {{ λ v, Φ v ∗ link_in_state Boundary }}.
+Proof using.
+  iIntros (Hislink) "Hlkst Hwp". iDestruct (wp_link_run_mut _ _ _ _ Hislink) as "[_ H]".
+  iApply ("H" with "Hwp Hlkst").
+Qed.
+
+Lemma wp_link_internal_call p fn vs (func: Link.func Λ1 Λ2) Φ E :
+  prog p !! fn = Some func →
+  (▷ WP LkSE (Link.RunFunction func vs) @ p; E {{ Φ }}) -∗
+  WP LkSE (Link.ExprCall fn vs) @ p; E {{ Φ }}.
+Proof using.
+  iIntros (Hfn) "Hwp".
+  rewrite (_: LkSE (Link.ExprCall fn vs) = of_class _ (ExprCall fn vs)) //.
+  by iApply wp_internal_call.
+Qed.
+
+Lemma wp_link_run_function1 p (func : Λ1.(func)) vs e1 Φ E :
+  apply_func func vs = Some e1 →
+  link_in_state Boundary -∗
+  ▷ (link_in_state In1 -∗ at_boundary Λ1 -∗
+      WP LkSE (Link.Expr1 e1) @ p; E {{ Φ }}) -∗
+  WP LkSE (Link.RunFunction (inl func) vs) @ p; E {{ Φ }}.
+Proof using.
+  iIntros (Hfunc) "(Hb & Hb1 & Hb2) Hwp". iApply wp_unfold. rewrite /wp_pre /=.
+  iIntros (σ) "Hσ".
+  iDestruct (link_at_boundary with "Hσ Hb") as %(pubσ & privσ1 & privσ2 & ->).
+  iDestruct "Hσ" as "(Hob & Hpub & Hpriv1 & Hpriv2)".
+  iMod (state_interp_join with "Hpub Hpriv1") as (σ1) "(Hσ1 & %Hsplit)".
+  iModIntro. iRight. iRight.
+  iSplitR.
+  { iPureIntro. eapply head_prim_reducible. exists (λ _, True). by econstructor. }
+  iIntros (X Hstep). apply head_reducible_prim_step in Hstep.
+  2: { exists (λ _, True). by econstructor. }
+  inversion Hstep; simplify_eq/=. simplify_split_state.
+  iMod (link_state_update _ In1 with "Hob Hb") as "[Hob Hb]".
+  iIntros "!>!>!>". iExists _, _. iSplitR; first done.
+  simpl. iFrame. iApply ("Hwp" with "[-Hb1] Hb1"). iFrame.
+Qed.
+
+Lemma wp_link_run_function2 p (func : Λ2.(func)) vs e2 Φ E :
+  apply_func func vs = Some e2 →
+  link_in_state Boundary -∗
+  ▷ (link_in_state In2 -∗ at_boundary Λ2 -∗
+      WP LkSE (Link.Expr2 e2) @ p; E {{ Φ }}) -∗
+  WP LkSE (Link.RunFunction (inr func) vs) @ p; E {{ Φ }}.
+Proof using.
+  iIntros (Hfunc) "(Hb & Hb1 & Hb2) Hwp". iApply wp_unfold. rewrite /wp_pre /=.
+  iIntros (σ) "Hσ".
+  iDestruct (link_at_boundary with "Hσ Hb") as %(pubσ & privσ1 & privσ2 & ->).
+  iDestruct "Hσ" as "(Hob & Hpub & Hpriv1 & Hpriv2)".
+  iMod (state_interp_join with "Hpub Hpriv2") as (σ2) "(Hσ2 & %Hsplit)".
+  iModIntro. iRight. iRight.
+  iSplitR.
+  { iPureIntro. eapply head_prim_reducible. exists (λ _, True). by econstructor. }
+  iIntros (X Hstep). apply head_reducible_prim_step in Hstep.
+  2: { exists (λ _, True). by econstructor. }
+  inversion Hstep; simplify_eq/=. simplify_split_state.
+  iMod (link_state_update _ In2 with "Hob Hb") as "[Hob Hb]".
+  iIntros "!>!>!>". iExists _, _. iSplitR; first done.
+  simpl. iFrame. iApply ("Hwp" with "[-Hb2] Hb2"). iFrame.
 Qed.
 
 End Linking_logic.
